feat: add new correct alpha_equiv todo: term_eqn failed to define

qcp/ast/annotated_C/alpha_equiv.c
@@ -121,19 +121,49 @@ bool alpha_equiv(term *t1, term *t2)
       if (strcmp(t1->content.Quant.var, t2->content.Quant.var) == 0) {
         return alpha_equiv(t1->content.Quant.body, t2->content.Quant.body);
       } else {
-        /*@ exists qv1 qv2,
-            store_string(t1 -> content.Quant.var, qv1) *
-            store_string(t2 -> content.Quant.var, qv2) 
+        /*@ 
+            exists y1 z1 qt1 qv1 qterm1 y2 z2 qt2 qv2 qterm2,
+              t1 != 0 && t2 != 0 &&
+              term1 == TermQuant(qt1, qv1, qterm1) &&
+              term2 == TermQuant(qt2, qv2, qterm2) &&
+              data_at(&(t1 -> type), termtypeID(term1)) *
+              data_at(&(t2 -> type), termtypeID(term2)) *
+              data_at(&(t1 -> content.Quant.type), qtID(qt1)) *
+              data_at(&(t2 -> content.Quant.type), qtID(qt2)) *
+              data_at(&(t1 -> content.Quant.var), y1) *
+              data_at(&(t2 -> content.Quant.var), y2) *
+              data_at(&(t1 -> content.Quant.body), z1) *
+              data_at(&(t2 -> content.Quant.body), z2) *
+              store_string(y1, qv1) * store_term(z1, qterm1) *
+              store_string(y2, qv2) * store_term(z2, qterm2)
             which implies
-            t1 -> content.Quant.var != 0 &&
-            t2 -> content.Quant.var != 0 &&
-            store_string(t1 -> content.Quant.var, qv1) *
-            store_string(t2 -> content.Quant.var, qv2) 
+              store_term(t1, term1) * store_term(t2, term2)
         */
-        term *t21 = subst_var(t1->content.Quant.var, t2->content.Quant.var, copy_term(t2->content.Quant.body));
-        bool result = alpha_equiv(t1->content.Quant.body, t21);
-        free_term(t21);
-        return result;
+        char *new_var = fresh(t1, t2);
+        /*@ 
+            store_term(t1, term1) * store_term(t2, term2)
+            which implies
+            exists y1 z1 qt1 qv1 qterm1 y2 z2 qt2 qv2 qterm2,
+              t1 != 0 && t2 != 0 &&
+              term1 == TermQuant(qt1, qv1, qterm1) &&
+              term2 == TermQuant(qt2, qv2, qterm2) &&
+              data_at(&(t1 -> type), termtypeID(term1)) *
+              data_at(&(t2 -> type), termtypeID(term2)) *
+              data_at(&(t1 -> content.Quant.type), qtID(qt1)) *
+              data_at(&(t2 -> content.Quant.type), qtID(qt2)) *
+              data_at(&(t1 -> content.Quant.var), y1) *
+              data_at(&(t2 -> content.Quant.var), y2) *
+              data_at(&(t1 -> content.Quant.body), z1) *
+              data_at(&(t2 -> content.Quant.body), z2) *
+              store_string(y1, qv1) * store_term(z1, qterm1) *
+              store_string(y2, qv2) * store_term(z2, qterm2)
+        */
+        term *new_t1 = subst_var(new_var, t1->content.Quant.var, copy_term(t1->content.Quant.body));
+        term *new_t2 = subst_var(new_var, t2->content.Quant.var, copy_term(t2->content.Quant.body));
+        bool result = alpha_equiv(new_t1, new_t2);
+        free_term(new_t1);
+        free_term(new_t2);
+        free_str(new_var);
       }
     }
   }
